Add typing proofs, half of semantics proofs for definition axioms
Prove definition axioms well-typed
(Some gen stuff for funpred_defs)
Working on semantics, proved t_insert equal lemma
Needed to assume pat match exhaustiveness, add
Almost done - need rep for gen alpha convert and gen_app

proofs/transform/eliminate_definition.v
@@ -22,6 +22,12 @@ Definition gen_sym_params {b: bool} (f: gen_sym b) : list typevar :=
   | false => s_params
   end f.
 
+Definition gen_sym_args {b: bool} (f: gen_sym b) : list vty :=
+  match b return gen_sym b -> list vty with
+  | true => s_args
+  | false => s_args
+  end f.
+
 Definition gen_funpred_def (b: bool) (f: gen_sym b) (l: list vsymbol) (t: gen_term b) : funpred_def :=
   match b return gen_sym b -> gen_term b -> funpred_def with
   | true => fun ls t => fun_def ls l t
@@ -33,6 +39,16 @@ Definition gen_funpred_def_match (x: funpred_def) : {b: bool & (gen_sym b * list
   | fun_def ls vs t => existT _ true (ls, vs, t)
   | pred_def ls vs f => existT _ false (ls, vs, f)
   end.
+
+Lemma gen_funpred_def_match_eq (x: funpred_def) b ls vs tms:
+  gen_funpred_def_match x = existT _ b (ls, vs, tms) <-> gen_funpred_def b ls vs tms = x.
+Proof.
+  unfold gen_funpred_def_match, gen_funpred_def. destruct x; simpl.
+  - split; intros Hex; [|destruct b]; inversion Hex; subst; auto.
+    apply inj_pair2_eq_dec in Hex; [inversion Hex; subst; auto | apply Bool.bool_dec].
+  - split; intros Hex; [|destruct b]; inversion Hex; subst; auto.
+    apply inj_pair2_eq_dec in Hex; [inversion Hex; subst; auto | apply Bool.bool_dec].
+Qed.
 
 (*Common features: let, match, app (fun or predsym), if*)
 Definition gen_app (b: bool) (f: gen_sym b) (tys: list vty) (tms: list term) : gen_term b :=
@@ -367,6 +383,627 @@ Proof.
     + rewrite axioms_of_def_elim. reflexivity.
     + destruct nonrec; [|reflexivity]. rewrite axioms_of_def_elim. reflexivity.
 Qed.
+
+(*Part 1: Everything is well-typed*)
+
+Print valid_def.
+Print funpred_valid.
+
+Section Typing.
+
+(* funpred_valid =
+fun (gamma : context) (l : list funpred_def) =>
+Forall (funpred_def_valid_type gamma) l /\
+funpred_def_term_exists gamma l
+
+| recursive_def fs => funpred_valid gamma fs
+| inductive_def l => indprop_valid gamma l
+| nonrec_def f =>
+    funpred_def_valid_type gamma f /\ nonrec_def_nonrec f *)
+
+Lemma t_insert_gen_typed gamma {b: bool} (ty: gen_type b) (t1 t2: gen_term b):
+  @gen_typed gamma b t1 ty ->
+  @gen_typed gamma b t2 ty ->
+  formula_typed gamma (t_insert_gen ty t1 t2).
+Proof.
+  (*Prove in 2 parts bc of induction*)
+  unfold gen_typed, gen_type, gen_term in *. destruct b; simpl in *.
+  - intros Hty1 Hty2.
+    apply (term_ind (fun t2 => forall ty t1 (Hty1: term_has_type gamma t1 ty) (Hty2: term_has_type gamma t2 ty),
+      formula_typed gamma (t_insert ty t1 t2)) (fun _ => True)); intros; simpl; auto; 
+        try solve[apply F_Eq; assumption]; inversion Hty3; subst; constructor; auto;
+    [| | rewrite null_map; assumption]; intros x; rewrite in_map_iff; intros [y [Hx Hiny]]; subst; simpl; auto.
+    rewrite Forall_map, Forall_forall in H0. auto.
+  - intros Hty1 Hty2.
+    apply (formula_ind (fun _ => True) (fun f2 => forall f1 (Hty1: formula_typed gamma f1) 
+      (Hty2: formula_typed gamma f2),
+      formula_typed gamma (f_insert f1 f2))); intros; simpl; auto; 
+        try solve[apply F_Eq; assumption]; inversion Hty3; subst; constructor; auto;
+    [| | rewrite null_map; assumption]; intros x; rewrite in_map_iff; intros [y [Hx Hiny]]; subst; simpl; auto.
+    rewrite Forall_map, Forall_forall in H0. auto.
+Qed.
+
+Check T_Fun.
+
+Definition gen_sig (b: bool) : context -> list (gen_sym b) :=
+  match b return context -> list (gen_sym b) with
+  | true => sig_f
+  | false => sig_p
+  end.
+
+Definition gen_valid_type {b: bool} (gamma: context) (ty: gen_type b) : Prop :=
+  match b return gen_type b -> Prop with
+  | true => fun ty => valid_type gamma ty
+  | false => fun _ => True
+  end ty.
+
+Definition gen_ty_subst {b: bool} (params: list typevar) (tys: list vty) (ty: gen_type b) : gen_type b :=
+  match b return gen_type b -> gen_type b with
+  | true => ty_subst params tys
+  | false => fun _ => tt
+  end ty.
+
+Lemma gen_app_typed {b: bool} gamma (ls: gen_sym b) (tys: list vty) (tms: list term) (ty: gen_type b)
+  (Inf: In ls (gen_sig b gamma))
+  (Hval: Forall (valid_type gamma) tys)
+  (Hvalret: gen_valid_type gamma (gen_sym_ret ls))
+  (* (Hlentms: length tms = length (gen_sym_args ls)) *)
+  (Hlentys: length tys = length (gen_sym_params ls))
+  (Hinner: Forall2 (term_has_type gamma) tms (map (ty_subst (gen_sym_params ls) tys) (gen_sym_args ls)))
+  (Hty: ty = gen_ty_subst (gen_sym_params ls) tys (gen_sym_ret ls))
+  : @gen_typed gamma b (gen_app b ls tys tms) ty.
+Proof.
+  rewrite Forall2_combine in Hinner.
+  destruct Hinner as [Htms Hinner]; rewrite map_length in Htms.
+  destruct b; simpl in *; subst; constructor; auto.
+Qed.
+
+Print valid_context.
+(* 
+Lemma axioms_of_def_typed gamma which (l: list funpred_def)
+  (Hall: Forall (funpred_def_valid_type gamma) l):
+  (* (Hinp: In (fst x) (sig_p gamma))
+  (Hallval: Forall (valid_type gamma) (s_args (fst x)))
+  (Hindform: Forall (valid_ind_form (fst x)) (map snd (snd x)))
+  (Htys: Forall (formula_typed gamma) (map snd (snd x)))*)
+  forall ax,
+  In ax (axioms_of_def which l) ->
+  formula_typed gamma (snd ax).
+Proof.
+  intros ax. unfold axioms_of_def. (*Nicer: concat instead of fold_right*) 
+  rewrite in_concat.
+  intros [axs [Hinaxs Hax]].
+  rewrite in_map_iff in Hinaxs.
+  destruct Hinaxs as [fd [Haxs Hinfd]]; subst.
+  destruct (gen_funpred_def_match fd) as [b [[ls vs] e]] eqn : Hgen; simpl in *.
+  destruct (which b ls) eqn : Hwhich; [| contradiction].
+  destruct Hax as [Hax | []]. subst. 
+  unfold rec_axiom. simpl.
+  apply fforalls_typed.
+  - apply t_insert_gen_typed.
+    + apply gen_app_typed.
+      unfold gen_funpred_def_match  in Hgen.
+      Print funpred_def_valid_type.
+  Search fforalls formula_typed.
+
+
+
+  simpl in Hax.
+  destruct (gen_funpred_def_match fd) *)
+  (*TODO: what conditions do we need on l?*)
+Check gen_funpred_def.
+Print funpred_def_valid_type.
+
+Definition gen_type_vars {b: bool} (t: gen_term b) : list typevar :=
+  match b return gen_term b -> list typevar with
+  | true => tm_type_vars
+  | false => fmla_type_vars
+  end t.
+
+Definition gen_funpred_def_valid_type gamma {b: bool} (ls: gen_sym b) (vs: list vsymbol)
+  (t: gen_term b):
+  funpred_def_valid_type gamma (gen_funpred_def b ls vs t) <->
+  @gen_typed gamma b t (gen_sym_ret ls) /\
+  sublist (gen_fv b t) vs /\
+  sublist (gen_type_vars t) (gen_sym_params ls) /\
+  NoDup (map fst vs) /\
+  map snd vs = gen_sym_args ls.
+Proof.
+  unfold gen_funpred_def. destruct b; simpl; reflexivity.
+Qed.
+
+(* Need to know that recursive function args are
+Lemma indprop_params_valid {gamma: context}
+  (gamma_valid: valid_context gamma)
+  {l: list indpred_def} {p: predsym} {fs: list (string * formula)}
+  (l_in: In (inductive_def l) gamma)
+  (def_in: In (ind_def p fs) l):
+  Forall (valid_type gamma) (s_args p). *)
+
+Definition wf_gen_sym {b: bool} gamma (ls: gen_sym b) : Prop :=
+  match b return gen_sym b -> Prop with
+  | true => wf_funsym gamma
+  | false => wf_predsym gamma
+  end ls.
+
+(*NOTE: don't care about type variables right now*)
+Lemma wf_gen_sym_valid {b: bool} {gamma} {ls: gen_sym b}
+  (Hwf: wf_gen_sym gamma ls):
+  Forall (valid_type gamma) (gen_sym_args ls) /\
+  gen_valid_type gamma (gen_sym_ret ls).
+Proof.
+  destruct b; simpl in *.
+  - unfold wf_funsym in Hwf. inversion Hwf as [ | ? ? [Hret _] Hargs]; subst.
+    split; auto. revert Hargs. apply Forall_impl. intros a Hval; apply Hval.
+  - split; auto.  unfold wf_predsym in Hwf. revert Hwf. apply Forall_impl. 
+    intros a Hval; apply Hval.
+Qed.
+
+(*TODO: move*)
+Lemma recpred_in_predsyms {gamma} {f: predsym} {l: list funpred_def}
+  (l_in: In l (mutfuns_of_context gamma))
+  (f_in: predsym_in_mutfun f l):
+  In f (predsyms_of_context gamma).
+Proof.
+  unfold predsyms_of_context. rewrite in_concat.
+  exists (predsyms_of_def (recursive_def l)).
+  split. rewrite in_map_iff. exists (recursive_def l).
+  split; auto. apply in_mutfuns in l_in; auto.
+  apply in_bool_In in f_in. auto.
+Qed.
+
+(*NOTE: only need that it is in fun/predsyms of context*)
+
+Definition sym_in_context {b: bool} (ls: gen_sym b) gamma : Prop :=
+  match b return gen_sym b -> Prop with
+  | true => fun f => In f (funsyms_of_context gamma)
+  | false => fun f => In f (predsyms_of_context gamma)
+  end ls.
+
+Lemma in_context_wf_gen_sym {b: bool} gamma{ls: gen_sym b}
+  (gamma_wf: wf_context gamma)
+  (Hin: sym_in_context ls gamma):
+  wf_gen_sym gamma ls.
+Proof.
+  apply wf_context_alt in gamma_wf.
+  destruct gamma_wf as [Hfun [Hpred _]].
+  rewrite Forall_forall in Hfun, Hpred.
+  destruct b; simpl in *; auto.
+Qed.
+(* 
+  (Hin1: In (recursive_def l) gamma)
+  (Hin2: In (gen_funpred_def b ls vs e) l):
+  wf_gen_sym gamma ls.
+Proof.
+  apply wf_context_alt in gamma_wf.
+  destruct gamma_wf as [Hfun [Hpred _]].
+  rewrite Forall_forall in Hfun, Hpred.
+  destruct b; simpl in *.
+  - apply Hfun. eapply recfun_in_funsyms.
+    + apply in_mutfuns, Hin1.
+    + eapply fun_in_mutfun. eauto.
+  - apply Hpred. eapply recpred_in_predsyms.
+    + apply in_mutfuns, Hin1.
+    + eapply pred_in_mutfun. eauto.
+Qed. *)
+
+Lemma recursive_def_in_gen_sig {b: bool} gamma  {ls: gen_sym b}
+  (Hin: sym_in_context ls gamma):
+  In ls (gen_sig b gamma).
+Proof.
+  pose proof (concrete_in_sig gamma) as [_ [Hfun Hpred]].
+  rewrite Forall_forall in Hfun, Hpred.
+  destruct b; simpl in *; auto.
+Qed.
+
+Lemma a_convert_gen_typed {b: bool} gamma (t: gen_term b) (vs: list vsymbol) (ty: gen_type b):
+  @gen_typed gamma b t ty ->
+  @gen_typed gamma b (a_convert_gen t vs) ty.
+Proof.
+  intros Hty. destruct b; simpl in *.
+  - apply a_convert_t_ty; assumption.
+  - apply a_convert_f_typed; assumption.
+Qed.
+
+Lemma recursive_in_context {b: bool} gamma {l: list funpred_def} {ls: gen_sym b}
+  {vs: list vsymbol} {e: gen_term b} 
+  (Hin1: In (recursive_def l) gamma)
+  (Hin2: In (gen_funpred_def b ls vs e) l):
+  sym_in_context ls gamma.
+Proof.
+  destruct b; simpl in *.
+  - eapply recfun_in_funsyms.
+    + apply in_mutfuns, Hin1.
+    + eapply fun_in_mutfun. eauto.
+  - eapply recpred_in_predsyms.
+    + apply in_mutfuns, Hin1.
+    + eapply pred_in_mutfun. eauto.
+Qed.
+
+Lemma nonrec_in_context {b: bool} gamma {ls: gen_sym b}
+  {vs: list vsymbol} {e: gen_term b} 
+  (Hin: In (nonrec_def (gen_funpred_def b ls vs e)) gamma):
+  sym_in_context ls gamma.
+Proof.
+  destruct b; simpl in *.
+  - eapply nonrec_in_funsyms; eauto.
+  - eapply nonrec_in_predsyms; eauto.
+Qed.
+
+Lemma gen_typevars_in_params {x v b} (ls: gen_sym b)
+  (Hinx: In x (gen_sym_args ls))
+  (Hinv: In v (type_vars x)):
+  In v (gen_sym_params ls).
+Proof.
+  destruct (In_nth _ _ vty_int Hinx) as [i [Hi Hx]]; subst.
+  destruct b; simpl in *; apply (typevars_in_params _ _ Hi _ Hinv).
+Qed.
+
+Lemma rec_axiom_typed {gamma b ls vs e}
+  (gamma_valid: valid_context gamma)
+  (Hallval: funpred_def_valid_type gamma (gen_funpred_def b ls vs e))
+  (Hinctx: sym_in_context ls gamma):
+  formula_typed gamma (snd (rec_axiom ls vs e)).
+Proof.
+  apply gen_funpred_def_valid_type in Hallval.
+  destruct Hallval as [Hty [Hsubvs [Hsubparams [Hnodup Hvs]]]].
+  assert (Hwf: wf_gen_sym gamma ls) (*NOTE: need this*)
+    by apply (in_context_wf_gen_sym gamma (valid_context_wf _ gamma_valid) Hinctx).
+  apply wf_gen_sym_valid in Hwf.
+  destruct Hwf as [Hvalargs Hvalret].
+  (*Now we can prove each part*)
+  apply fforalls_typed.
+  2: { rewrite <- Forall_map. rewrite Hvs. apply Hvalargs. }
+  apply t_insert_gen_typed.
+  2: { apply a_convert_gen_typed, Hty. }
+  apply gen_app_typed; auto.
+  + apply (recursive_def_in_gen_sig _ Hinctx).
+  + rewrite Forall_map. rewrite Forall_forall. intros x Hinsym. constructor.
+  + rewrite map_length; reflexivity.
+  + (*The nontrivial part: prove that the arguments are correct*)
+    rewrite map_id'.
+    2: {
+      rewrite Forall_forall. intros x Hinx.
+      apply ty_subst_params_id.
+      intros v Hinv.
+      eapply gen_typevars_in_params. apply Hinx. auto.
+    }
+    replace vs with (combine (map fst vs) (gen_sym_args ls)).
+    2: { rewrite <- Hvs, combine_eq. reflexivity. }
+    rewrite Forall2_nth.
+    assert (Hvslen: length vs = length (gen_sym_args ls)). {
+      rewrite <- Hvs, map_length; reflexivity.
+    }
+    split; unfold vsymbol in *; rewrite map_length, combine_length, map_length, Hvslen, Nat.min_id; [reflexivity|].
+    intros i d1 d2 Hi. rewrite map_nth_inbound with (d2:=(""%string, vty_int));
+    [| rewrite combine_length, map_length; lia].
+    apply T_Var'; auto.
+    * rewrite Forall_nth in Hvalargs. auto.
+    * rewrite combine_nth; [| rewrite map_length; lia]. simpl. apply nth_indep, Hi.
+  + (*And return type*)
+    (*Just case on b*)
+    destruct b; simpl in *; auto.
+    symmetry; apply ty_subst_params_id.
+    intros v Hinv.
+    assert (ls_wf: check_sublist (type_vars (f_ret ls)) (s_params ls)) by (destruct ls; auto).
+    apply (reflect_iff _ _ (check_sublist_correct _ _) ) in ls_wf.
+    apply ls_wf, Hinv.
+Qed.
+
+Lemma gen_axioms_typed which (nonrec : bool) (t: task) (t_wf: task_wf t):
+forall fmla : formula,
+In fmla (map snd (concat (map (fun x =>
+    match x with
+    | recursive_def l => rev (axioms_of_def which l)
+    | nonrec_def l => if nonrec then rev (axioms_of_def which [l]) else nil
+    | _ => []
+    end) (task_gamma t)))) -> formula_typed (task_gamma t) fmla.
+Proof.
+  rewrite <- Forall_forall, Forall_map, Forall_concat, Forall_map.
+  rewrite Forall_forall; intros d Hd.
+  rewrite Forall_forall; intros ax.
+  destruct d; try solve[intros []].
+  - rewrite <- In_rev. (*LOTS of boilerplate should reduce*)
+    unfold axioms_of_def. (*Nicer: concat instead of fold_right*) 
+    rewrite in_concat.
+    intros [axs [Hinaxs Hax]].
+    rewrite in_map_iff in Hinaxs.
+    destruct Hinaxs as [fd [Haxs Hinfd]]; subst.
+    destruct (gen_funpred_def_match fd) as [b [[ls vs] e]] eqn : Hgen; simpl in *.
+    destruct (which b ls) eqn : Hwhich; [| contradiction].
+    destruct Hax as [Hax | []]. subst. 
+    apply gen_funpred_def_match_eq in Hgen. subst.
+    inversion t_wf.
+    pose proof (valid_context_defs _ task_gamma_valid) as Hallval.
+    rewrite Forall_forall in Hallval.
+    specialize (Hallval _ Hd).
+    simpl in Hallval.
+    unfold funpred_valid in Hallval.
+    destruct Hallval as [Hallval Hterm]. (*TODO: do we need termination? maybe I was right?*)
+    rewrite Forall_forall in Hallval.
+    specialize (Hallval _ Hinfd).
+    assert (Hinctx: sym_in_context ls (task_gamma t)) by
+          apply (recursive_in_context _ Hd Hinfd).
+    apply rec_axiom_typed; assumption.
+  - destruct nonrec; [|contradiction].
+    unfold axioms_of_def.
+    rewrite <- In_rev, in_concat. 
+    simpl. intros [axs [[Hinaxs | []] Hax]].
+    destruct (gen_funpred_def_match f) as [b [[ls vs] e]] eqn : Hgen; simpl in *.
+    destruct (which b ls) eqn : Hwhich; [| subst; contradiction]. subst.
+    destruct Hax as [Hax | []]. subst. 
+    unfold rec_axiom. simpl.
+    apply gen_funpred_def_match_eq in Hgen. subst.
+    inversion t_wf.
+    pose proof (valid_context_defs _ task_gamma_valid) as Hallval.
+    rewrite Forall_forall in Hallval.
+    specialize (Hallval _ Hd).
+    simpl in Hallval.
+    destruct Hallval as [Hallval Hterm].
+    assert (Hinctx: sym_in_context ls (task_gamma t)) by
+          apply (nonrec_in_context _ Hd).
+    apply rec_axiom_typed; assumption.
+Qed.
+
+(*Part 2: Axioms are sound*)
+From Equations Require Import Equations.
+
+Ltac split_all_dec_eq :=
+  match goal with
+  | |- @eq bool (proj_sumbool _ _ (all_dec (?x = ?y)))  (proj_sumbool _ _ (all_dec (?a = ?b))) => 
+    let H1 := fresh in let H2 := fresh in
+    assert (H1: x = a); [| assert (H2: y = b); [| rewrite H1, H2]]
+  end.
+    
+Lemma sublist_cons {A: Type} (l1 l2 : list A) x:
+  sublist l1 l2 ->
+  sublist l1 (x :: l2).
+Proof.
+  unfold sublist. simpl. intros. right; auto.
+Qed.
+
+(*A key result: t_insert_gen*)
+(*It must be the case that the free vars of t1 do not intersect with the boundvars of t2*)
+Lemma t_insert_rep {gamma} (gamma_valid: valid_context gamma) pd vt pf vv ty t1 t2 Hty Hty1 Hty2
+  (Hdisj: disj (tm_fv t1) (tm_bnd t2)):
+  formula_rep gamma_valid pd vt pf vv (t_insert ty t1 t2) Hty =
+  all_dec (term_rep gamma_valid pd vt pf vv t1 ty Hty1 =
+    term_rep gamma_valid pd vt pf vv t2 ty Hty2).
+Proof.
+  revert vv t1 Hdisj Hty Hty1 Hty2.
+  apply (term_ind (fun t2 => forall vv t1,
+    disj (tm_fv t1) (tm_bnd t2) ->
+    forall Hty Hty1 Hty2,
+    formula_rep gamma_valid pd vt pf vv
+    (t_insert ty t1 t2) Hty =
+  all_dec
+    (term_rep gamma_valid pd vt pf vv t1 ty Hty1 =
+  term_rep gamma_valid pd vt pf vv t2 ty Hty2)) (fun _ => True)); simpl; intros; simpl_rep_full; auto.
+  - split_all_dec_eq; auto; apply term_rep_irrel.
+  - split_all_dec_eq; auto; [apply term_rep_irrel | apply dom_cast_eq].
+  - split_all_dec_eq; auto; [apply term_rep_irrel |].
+    unfold fun_arg_list. erewrite get_arg_list_eq.
+    unfold cast_dom_vty. rewrite !dom_cast_compose. apply dom_cast_eq.
+    rewrite Forall_forall; intros; apply term_rep_irrel.
+  - (*First interesting case: Tlet*)
+    rewrite H0 with (Hty1:=Hty1) (Hty2:=(proj2' (ty_let_inv Hty2))).
+    2: { eapply disj_sublist. apply H1. apply sublist_cons. apply sublist_app_r. }
+    (*Use disj*)
+    rewrite tm_change_vv with (v2:=vv); auto.
+    + erewrite (term_rep_irrel _ _ _ _ _ tm1). reflexivity.
+    + intros x Hinx. unfold substi. destruct (vsymbol_eq_dec x v); subst; auto.
+      exfalso. apply (H1 v); split; simpl; auto.
+  - (*Tif*)
+    rewrite fmla_rep_irrel with (Hval2:= (proj2' (proj2' (ty_if_inv Hty2)))).
+    destruct (formula_rep _ _ _ _ _ f _) eqn : Hrep.
+    + erewrite H0; [reflexivity|].
+      eapply disj_sublist. apply H2. eapply sublist_trans. apply sublist_app_l.
+      apply sublist_app_r.
+    + erewrite H1; [reflexivity|].
+      eapply disj_sublist. apply H2. rewrite app_assoc. apply sublist_app_r.
+  - (*Tmatch*)
+    rewrite term_rep_irrel with (Hty2:=(proj1' (ty_match_inv Hty2))).
+    generalize dependent (proj1' (proj2' (typed_match_inv Hty))).
+    generalize dependent (proj2' (proj2' (typed_match_inv Hty))).
+    generalize dependent (proj1' (proj2' (ty_match_inv Hty2))).
+    generalize dependent (proj2' (proj2' (ty_match_inv Hty2))).
+    generalize dependent (term_rep gamma_valid pd vt pf vv tm v
+      (proj1' (ty_match_inv Hty2))).
+    (*Get hypotheses we need*)
+    clear -H0 H1. (*do we need Hty2/info about pattern typing?*)
+    induction ps as [|phd ptl IH]; simpl.
+    (*TODO: we actually need non-exhaustiveness here*)
+    + admit.
+    + intros d Hall1 Hall2 Hall3 Hall4.
+      destruct phd as [phd tdh]; simpl in *.
+      rewrite match_val_single_irrel with (Hval2:=(Forall_inv Hall2)).
+      simpl.
+      destruct (match_val_single gamma_valid pd vt v phd
+        (Forall_inv Hall2) d) as [l1|] eqn : Hmatch.
+      * (*use original IH*) rewrite Forall_forall in H0; rewrite H0 with (Hty1:=Hty1)(Hty2:=Forall_inv Hall1); simpl; auto.
+        -- rewrite tm_change_vv with (t:=t1)(v2:=vv); [reflexivity|].
+          intros x Hinx. rewrite extend_val_notin; auto.
+          rewrite <- (match_val_single_free_var _ _ _ _ _ _ _ _ _ Hmatch).
+          intros Hinx1.
+          apply (H1 x); split; auto. rewrite !in_app_iff; auto.
+        -- eapply disj_sublist. apply H1. eapply sublist_trans. apply sublist_app_r.
+          eapply sublist_trans. apply sublist_app_l. apply sublist_app_r.
+      * (*Use IH*) apply IH.
+        -- inversion H0; subst; auto.
+        -- eapply disj_sublist. apply H1. unfold sublist. intros x. rewrite !in_app_iff.
+          intros; destruct_all; auto.
+  - (*epsilon*)
+    split_all_dec_eq; auto; [ apply term_rep_irrel|].
+    f_equal. repeat (apply functional_extensionality_dep; intros).
+    erewrite fmla_rep_irrel.
+    erewrite fmla_change_vv. reflexivity.
+    intros y Hiny. unfold substi. destruct (vsymbol_eq_dec y v); subst; auto.
+    unfold eq_sym; simpl. apply dom_cast_eq.
+Admitted.
+
+(*And the same for formulas - can we prove easier?*)
+Lemma f_insert_rep {gamma} (gamma_valid: valid_context gamma) pd vt pf vv f1 f2 Hty Hty1 Hty2
+  (Hdisj: disj (fmla_fv f1) (fmla_bnd f2)):
+  formula_rep gamma_valid pd vt pf vv (f_insert f1 f2) Hty =
+  eqb (formula_rep gamma_valid pd vt pf vv f1 Hty1)
+    (formula_rep gamma_valid pd vt pf vv f2 Hty2).
+Proof.
+  revert vv f1 Hdisj Hty Hty1 Hty2.
+  apply (formula_ind (fun _ => True) (fun f2 => forall vv f1,
+    disj (fmla_fv f1) (fmla_bnd f2) ->
+    forall Hty Hty1 Hty2,
+    formula_rep gamma_valid pd vt pf vv
+    (f_insert f1 f2) Hty =
+  eqb
+    (formula_rep gamma_valid pd vt pf vv f1 Hty1)
+  (formula_rep gamma_valid pd vt pf vv f2 Hty2))); simpl; intros; simpl_rep_full; auto;
+  try solve[f_equal; try solve[apply fmla_rep_irrel]; auto; 
+    solve[repeat(f_equal; auto; apply fmla_rep_irrel)]].
+  - (*Fpred*)
+    f_equal; [apply fmla_rep_irrel |f_equal]. apply get_arg_list_eq.
+    rewrite Forall_forall; intros; apply term_rep_irrel.
+  - (*Feq*) f_equal; [apply fmla_rep_irrel|].
+    split_all_dec_eq; [| | reflexivity]; apply term_rep_irrel.
+  - (*Flet*) 
+    rewrite H0 with (Hty1:=Hty1)(Hty2:=(proj2' (typed_let_inv Hty2))).
+    2: { eapply disj_sublist. apply H1. apply sublist_cons. apply sublist_app_r. }
+    (*Use disj*)
+    rewrite fmla_change_vv with (v2:=vv); auto.
+    + erewrite (term_rep_irrel _ _ _ _ _ tm). reflexivity.
+    + intros x Hinx. unfold substi. destruct (vsymbol_eq_dec x v); subst; auto.
+      exfalso. apply (H1 v); split; simpl; auto.
+  - (*Fif*)
+    rewrite fmla_rep_irrel with (Hval2:= (proj1' (typed_if_inv Hty2))).
+    destruct (formula_rep _ _ _ _ _ f1 _) eqn : Hrep.
+    + erewrite H0; [reflexivity|].
+      eapply disj_sublist. apply H2. eapply sublist_trans. apply sublist_app_l.
+      apply sublist_app_r.
+    + erewrite H1; [reflexivity|].
+      eapply disj_sublist. apply H2. rewrite app_assoc. apply sublist_app_r.
+  - (*Fmatch*)
+    rewrite term_rep_irrel with (Hty2:=(proj1' (typed_match_inv Hty2))).
+    generalize dependent (proj1' (proj2' (typed_match_inv Hty))).
+    generalize dependent (proj2' (proj2' (typed_match_inv Hty))).
+    generalize dependent (proj1' (proj2' (typed_match_inv Hty2))).
+    generalize dependent (proj2' (proj2' (typed_match_inv Hty2))).
+    generalize dependent (term_rep gamma_valid pd vt pf vv tm v
+      (proj1' (typed_match_inv Hty2))).
+    clear -H0 H1. 
+    induction ps as [|phd ptl IH]; simpl.
+    (*TODO: we actually need non-exhaustiveness here*)
+    + admit.
+    + intros d Hall1 Hall2 Hall3 Hall4.
+      destruct phd as [phd tdh]; simpl in *.
+      rewrite match_val_single_irrel with (Hval2:=(Forall_inv Hall2)).
+      simpl.
+      destruct (match_val_single gamma_valid pd vt v phd
+        (Forall_inv Hall2) d) as [l1|] eqn : Hmatch.
+      * (*use original IH*) rewrite Forall_forall in H0; rewrite H0 with (Hty1:=Hty1)(Hty2:=Forall_inv Hall1); simpl; auto.
+        -- rewrite fmla_change_vv with (f:=f1)(v2:=vv); [reflexivity|].
+          intros x Hinx. rewrite extend_val_notin; auto.
+          rewrite <- (match_val_single_free_var _ _ _ _ _ _ _ _ _ Hmatch).
+          intros Hinx1.
+          apply (H1 x); split; auto. rewrite !in_app_iff; auto.
+        -- eapply disj_sublist. apply H1. eapply sublist_trans. apply sublist_app_r.
+          eapply sublist_trans. apply sublist_app_l. apply sublist_app_r.
+      * (*Use IH*) apply IH.
+        -- inversion H0; subst; auto.
+        -- eapply disj_sublist. apply H1. unfold sublist. intros x. rewrite !in_app_iff.
+          intros; destruct_all; auto.
+Admitted.
+
+Definition gen_bnd {b: bool} (t: gen_term b) : list vsymbol :=
+  match b return gen_term b -> list vsymbol with
+  | true => tm_bnd
+  | false => fmla_bnd
+  end t.
+
+Lemma all_dec_eqb (b1 b2: bool):
+  proj_sumbool _ _ (all_dec (b1 = b2)) = eqb b1 b2.
+Proof.
+  destruct (all_dec (b1 = b2)); subst; simpl.
+  - destruct b2; reflexivity.
+  - destruct b1; destruct b2; auto.
+Qed.
+
+Lemma t_insert_gen_rep {gamma} (gamma_valid: valid_context gamma) pd vt pf vv {b: bool}
+  (t1 t2: gen_term b) (ty: gen_type b) Hty Hty1 Hty2
+  (Hdisj: disj (gen_fv b t1) (gen_bnd t2)):
+  formula_rep gamma_valid pd vt pf vv (t_insert_gen ty t1 t2) Hty =
+  all_dec (gen_rep gamma_valid pd pf vt b vv ty t1 Hty1 = gen_rep gamma_valid pd pf vt b vv ty t2 Hty2).
+Proof.
+  destruct b; simpl.
+  - apply t_insert_rep; auto.
+  - rewrite all_dec_eqb. apply f_insert_rep; auto.
+Qed.
+
+
+Theorem gen_axioms_sound which nonrec : sound_trans (single_trans (gen_axioms which nonrec)).
+Proof.
+  apply add_axioms_sound.
+  - apply gen_axioms_typed.
+  - intros.
+    (*Now the hard part - show log conseq*)
+    unfold log_conseq_gen.
+    intros.
+    assert (Hfull:=pf_full).
+    destruct Hfull as [Hfun [Hpred _]].
+    unfold satisfies.
+    intros.
+    (*First, get more info about fmla*)
+    rewrite in_map_iff in H.
+    destruct H as [ax [Hfmla Hinax]]; subst.
+    rewrite in_concat in Hinax.
+    destruct Hinax as [constrs [Hinconstrs Hinax]]; subst.
+    rewrite in_map_iff in Hinconstrs.
+    destruct Hinconstrs as [d [Hconstrs Hind]]; subst.
+    (*TODO: again, see what we need*)
+    (*HERE*)
+    destruct d; try contradiction. 
+    + unfold axioms_of_def in Hinax.
+      rewrite <- In_rev, in_concat in Hinax.
+      destruct Hinax as [axs [Hinaxs Hinax]].
+      rewrite in_map_iff in Hinaxs.
+      destruct Hinaxs as [fd [Haxs Hinfd]].
+      destruct (gen_funpred_def_match fd) as [b [[ls vs] e]] eqn : Hgen; simpl in *. subst.
+      destruct (which b ls) eqn : Hwhich; [| subst; contradiction].
+      apply gen_funpred_def_match_eq in Hgen. subst.
+      destruct Hinax as [Hinax | []]; subst.
+      (*Here is the lemma we want - probably want func_defined or something *)
+      (*HERE*)
+      unfold rec_axiom. simpl.
+
+      (*need for [fforalls_rep]*)
+      assert (Hty1: formula_typed (task_gamma t)
+        (t_insert_gen (gen_sym_ret ls)
+        (gen_app b ls (map vty_var (gen_sym_params ls))
+        (map Tvar vs))
+        (a_convert_gen e vs))).
+      { unfold rec_axiom in Hty; simpl in Hty.
+        apply fforalls_typed_inv in Hty; apply Hty.
+      }
+      rewrite fforalls_rep' with (Hval1:=Hty1).
+      apply simpl_all_dec. intros h.
+      erewrite t_insert_gen_rep.
+
+      Unshelve.
+      erewrite fmla_rep_irrel.
+      rewrite fforalls_rep.
+      Unshelve.
+      2
+
+
+      rewrite in_
+    -
+
+
+
+
+    destruct d; try solve[inversion Hinax].
+    rewrite <- In_rev in Hinax.
+    unfold build_ind_axioms in Hinax.
+    rewrite in_app_iff in Hinax.
+    destruct Hinax as [Hinconstr | Hinax]. intros.
 
 
 (*Prove soundness*)
